Beginnings of HMAC implementation.

lush/Crypto/HMAC.lean
@@ -4,6 +4,61 @@ namespace Lush.Crypto.HMAC
 
 open Std
 open BitVec
+open Lush.Crypto.SHA
 
+def blockLengthBytes := 64
+
+def prepKey (key : ByteArray) (hlen : key.size < 2^61) : ByteArray :=
+  let key :=
+    if key.size ≤ blockLengthBytes
+    then key
+    else bitVecToByteArray (SHA.sha256 key hlen)
+  let zeroPaddingLen := blockLengthBytes - key.size
+  let zeroPadding := Array.replicate zeroPaddingLen 0 |> ByteArray.mk
+  key ++ zeroPadding
+
+def prep_key_size (key : ByteArray) (hlen : key.size < 2^61) :
+    (prepKey key hlen).size = blockLengthBytes := by
+  sorry
+
+def ipad : ByteArray :=
+  Array.replicate blockLengthBytes 0x36 |> ByteArray.mk
+
+theorem size_ipad : ipad.size = blockLengthBytes := by
+  simp [ipad]
+  rw [←ByteArray.size_data, Array.size_replicate]
+
+def opad : ByteArray :=
+  Array.replicate blockLengthBytes 0x5C |> ByteArray.mk
+
+theorem size_opad : opad.size = blockLengthBytes := by
+  simp [opad]
+  rw [←ByteArray.size_data, Array.size_replicate]
+
+/-
+TODO:
+ - I need an easier way to do bitwise operations on ByteArrays.
+ - Lemma for lengths of bytearray <-> bitvec conversions.
+ - The length lemmas are annoying, maybe I just skip them? I'll silently
+   create "wrong" hashes but they are still usable hashes, just non-compliant
+   with the RFC.
+-/
+
+def sha256hmac
+    (message : ByteArray)
+    (key : ByteArray)
+    (hlenmsg : message.size < 2^60)
+    (hlenkey : key.size < 2^61) :
+    ByteArray :=
+  let key := prepKey key hlenkey
+  let keyIpad :=
+    ((byteArrayToBitVec key).cast (by sorry) : BitVec (8 * blockLengthBytes))
+    ^^^ (byteArrayToBitVec ipad).cast (by sorry)
+  let keyOpad :=
+    ((byteArrayToBitVec key).cast (by sorry) : BitVec (8 * blockLengthBytes))
+    ^^^ (byteArrayToBitVec opad).cast (by sorry)
+  let innerHash := sha256 (bitVecToByteArray keyIpad ++ message) (by sorry)
+  let outerHash := sha256 (bitVecToByteArray keyOpad ++ bitVecToByteArray innerHash) (by sorry)
+  bitVecToByteArray outerHash
 
 end Lush.Crypto.HMAC
